# Surds

## Properties

$$
\begin{align*}
  \sqrt{a} + \sqrt{b} &\rightarrow \text{cannot be simplified} \\
  m\sqrt{a} + n\sqrt{a} &= (m+n)\sqrt{a}
\end{align*}
$$

### Rationalising the denominator

$$
\begin{align*}
  \frac{1}{\sqrt{a}} \cdot \frac{\sqrt{a}}{\sqrt{a}} &= \frac{\sqrt{a}}{a} \\
  \frac{1}{\sqrt{a} + \sqrt{b}} \cdot \frac{\sqrt{a} - \sqrt{b}}{\sqrt{a} - \sqrt{b}} &= \frac{\sqrt{a} - \sqrt{b}}{a - b} \\
  \frac{1}{\sqrt{a} - \sqrt{b}} \cdot \frac{\sqrt{a} + \sqrt{b}}{\sqrt{a} + \sqrt{b}} &= \frac{\sqrt{a} + \sqrt{b}}{a - b}
\end{align*}
$$
